Shift0Dollar/Simplified/FineGrained.v
@@ -45,12 +45,12 @@ Admitted.
 (* ANCHOR Decompose
  *)
 (* Decompose `w $ e` term, which is never stuck and always returns `dec_redex` with an empty context `K` *)
-Fixpoint decompose_delimited (w : val ␀) (e : tm ␀) : (T' ␀ * redex' ␀) :=
+Fixpoint decompose_delimited (w : val ∅) (e : tm ∅) : (T' ∅ * redex' ∅) :=
   match e with
   | tm_val v => (T_nil', redex_dollar' w v)  (* w $ v *)
   | tm_non p => decompose_delimitedP w p
   end
-with decompose_delimitedP (w : val ␀) (p : non ␀) : (T' ␀ * redex' ␀) :=
+with decompose_delimitedP (w : val ∅) (p : non ∅) : (T' ∅ * redex' ∅) :=
   match p with
   | <{ v v' }> =>
     match v with
@@ -62,12 +62,12 @@ with decompose_delimitedP (w : val ␀) (p : non ␀) : (T' ␀ * redex' ␀) :=
   | <{ let e in e' }> => (T_nil', redex_dol_let' w e e')                        (* w $ let e in e' *)
   end.
 
-Fixpoint decompose' (e : tm ␀) : dec T' redex' ␀ :=
+Fixpoint decompose' (e : tm ∅) : dec T' redex' ∅ :=
   match e with
   | tm_val v => dec_value v
   | tm_non p => decomposeP' p
   end
-with decomposeP' (p : non ␀) : dec T' redex' ␀ :=
+with decomposeP' (p : non ∅) : dec T' redex' ∅ :=
   match p with
   | <{ v v' }> =>
     match v with
@@ -87,7 +87,7 @@ with decomposeP' (p : non ␀) : dec T' redex' ␀ :=
 
 (* ANCHOR Evaluation
  *)
-Definition contract' (r : redex' ␀) : tm ␀ :=
+Definition contract' (r : redex' ∅) : tm ∅ :=
     match r with
     (* (λ x. e) v  ~>  e [x := v] *)
     | redex_beta' e v => <{ e [0 := v] }>
@@ -115,14 +115,14 @@ Definition optional_step' e :=
   end.
 
 Reserved Notation "e1 ~>' e2" (at level 40).
-Inductive contr' : tm ␀ → tm ␀ → Prop :=
+Inductive contr' : tm ∅ → tm ∅ → Prop :=
 | contr_tm' : ∀ r, redex_to_term' r ~>' contract' r
 where "e1 ~>' e2" := (contr' e1 e2).
 Global Hint Constructors contr' : core.
 
 Reserved Notation "e1 -->' e2" (at level 40).
-Inductive step' : tm ␀ → tm ␀ → Prop :=
-| step_tm' : ∀ (k : K ␀) (t : T' ␀) (e1 e2 : tm ␀), e1 ~>' e2 → <{ k[t[e1]] }> -->' <{ k[t[e2]] }>
+Inductive step' : tm ∅ → tm ∅ → Prop :=
+| step_tm' : ∀ (k : K ∅) (t : T' ∅) (e1 e2 : tm ∅), e1 ~>' e2 → <{ k[t[e1]] }> -->' <{ k[t[e2]] }>
 where "e1 -->' e2" := (step' e1 e2).
 Global Hint Constructors step' : core.
 
@@ -149,13 +149,97 @@ Lemma multi_contr_multi' : ∀ {e1 e2 e3},
 Proof.
   intros. eapply multi_step; try eapply (step_tm' K_nil T_nil'); cbn; eassumption.
 Qed.
-Definition contr_beta' : ∀ e (v : val ␀), <{ (λ e) v }> ~>' <{ e [ 0 := v ] }> := λ e v, contr_tm' (redex_beta' e v).
-Definition contr_dollar' : ∀ (v1 v2 : val ␀), <{ v1 $ v2 }> ~>' <{ v1 v2 }> := λ v1 v2, contr_tm' (redex_dollar' v1 v2).
-Definition contr_let_beta' : ∀ (v : val ␀) e, <{ let v in e }> ~>' <{ e [ 0 := v ] }> := λ v e, contr_tm' (redex_let_beta' v e).
-(* Definition contr_shift' : ∀ (w : val ␀) (v : val ␀), <{ w $ S₀ v }> ~>' <{ v w }> := λ w v, contr_tm' (redex_shift' w v). *)
-Definition contr_shift' : ∀ (w : val ␀) (v : val ␀), <{ w $ S₀ v }> ~>' <{ v (λ ↑w $ 0) }> := λ w v, contr_tm' (redex_shift' w v).
-Definition contr_dol_let' : ∀ (w : val ␀) e e', <{ w $ let e in e' }> ~>' <{ (λ ↑w $ e') $ e }> := λ w e e', contr_tm' (redex_dol_let' w e e').
+Definition contr_beta' : ∀ e (v : val ∅), <{ (λ e) v }> ~>' <{ e [ 0 := v ] }> := λ e v, contr_tm' (redex_beta' e v).
+Definition contr_dollar' : ∀ (v1 v2 : val ∅), <{ v1 $ v2 }> ~>' <{ v1 v2 }> := λ v1 v2, contr_tm' (redex_dollar' v1 v2).
+Definition contr_let_beta' : ∀ (v : val ∅) e, <{ let v in e }> ~>' <{ e [ 0 := v ] }> := λ v e, contr_tm' (redex_let_beta' v e).
+(* Definition contr_shift' : ∀ (w : val ∅) (v : val ∅), <{ w $ S₀ v }> ~>' <{ v w }> := λ w v, contr_tm' (redex_shift' w v). *)
+Definition contr_shift' : ∀ (w : val ∅) (v : val ∅), <{ w $ S₀ v }> ~>' <{ v (λ ↑w $ 0) }> := λ w v, contr_tm' (redex_shift' w v).
+Definition contr_dol_let' : ∀ (w : val ∅) e e', <{ w $ let e in e' }> ~>' <{ (λ ↑w $ e') $ e }> := λ w e e', contr_tm' (redex_dol_let' w e e').
 Global Hint Resolve step_contr' contr_beta' contr_dollar' contr_shift' contr_dol_let' contr_let_beta' : core.
+
+
+Lemma step_let' : ∀ {e1 e2 e},
+  e1 -->' e2 →
+  <{ let e1 in e }> -->' <{ let e2 in e }>.
+Proof.
+  intros. generalize dependent e.
+  induction H; auto; intros.
+  apply (step_tm' (K_let k e) t e1 e2).
+  apply H.
+Qed.
+
+Lemma multi_let' : ∀ {e1 e2 e},
+  e1 -->'* e2 →
+  <{ let e1 in e }> -->'* <{ let e2 in e }>.
+Proof.
+  intros. generalize dependent e.
+  induction H; auto; intros.
+  eapply (multi_step); [idtac | apply IHmulti].
+  apply step_let'.
+  apply H.
+Qed.
+
+(* Lemma step_delim' : ∀ {v : val ∅} {e1 e2},
+  e1 -->' e2 →
+  <{ v $ e1 }> -->' <{ v $ e2 }>.
+Proof.
+  intros. generalize dependent v.
+  induction H; auto; intros.
+  apply (step_tm' K_nil (T_cons' v k t) e1 e2).
+  apply H.
+Qed. *)
+
+(* Lemma multi_delim' : ∀ {v : val ∅} {e1 e2},
+  e1 -->'* e2 →
+  <{ v $ e1 }> -->'* <{ v $ e2 }>.
+Proof.
+  intros. generalize dependent v.
+  induction H; auto; intros.
+  eapply (multi_step); [idtac | apply IHmulti].
+  apply step_delim'.
+  apply H.
+Qed. *)
+
+Lemma step_k' : ∀ {e1 e2} {k : K ∅},
+  e1 -->' e2 →
+  <{ k[e1] }> -->' <{ k[e2] }>.
+Proof.
+  intros e1 e2 k; generalize dependent e1; generalize dependent e2.
+  induction k; auto; intros.
+  cbn. apply step_let'. apply IHk. apply H.
+Qed.
+
+Lemma multi_k' : ∀ {e1 e2} {k : K ∅},
+  e1 -->'* e2 →
+  <{ k[e1] }> -->'* <{ k[e2] }>.
+Proof.
+  intros. generalize dependent k.
+  induction H; auto; intros.
+  eapply (multi_step); [idtac | apply IHmulti].
+  apply step_k'.
+  apply H.
+Qed.
+
+(* Lemma step_t' : ∀ {e1 e2} {t : T' ∅},
+  e1 -->' e2 →
+  <{ t[e1] }> -->' <{ t[e2] }>.
+Proof.
+  intros e1 e2 t; generalize dependent e1; generalize dependent e2.
+  induction t; auto; intros.
+  cbn. apply step_delim'. apply step_k'. apply IHt. apply H.
+Qed.
+
+Lemma multi_t' : ∀ {e1 e2} {t : T' ∅},
+  e1 -->'* e2 →
+  <{ t[e1] }> -->'* <{ t[e2] }>.
+Proof.
+  intros. generalize dependent t.
+  induction H; auto; intros.
+  eapply (multi_step); [idtac | apply IHmulti].
+  apply step_t'.
+  apply H.
+Qed. *)
+
 
 Lemma deterministic_contr' : ∀ e e1 e2,
   e ~>' e1 →
@@ -204,13 +288,13 @@ Fixpoint eval' i e :=
   end.
 
 Section Examples.
-  Definition _id : val ␀ := <{ λ 0 }>.
-  Definition _const : val ␀ := <{ λ λ 1 }>.
+  Definition _id : val ∅ := <{ λ 0 }>.
+  Definition _const : val ∅ := <{ λ λ 1 }>.
 
   Compute (eval' 10 <{ _id $ _const $ S₀ (λ 0) }>).
   Compute (eval' 10 <{ _const $ _id $ S₀ (λ 0) }>).
 
-  Definition _e1 : tm ␀ := <{
+  Definition _e1 : tm ∅ := <{
     _id $
       let λ 0 0 in
       let S₀ 0 in
