Common.v
@@ -11,8 +11,8 @@ Notation "V ↑ n" := (iter Type n option V) (at level 5, left associativity) : 
 Notation "^ V" := (option V) (at level 4, right associativity) : type_scope.
 
 Inductive Void : Type := .
-Notation "␀" := (Void).
-Definition from_void {A} (v : ␀) : A := match v with end.
+Notation "∅" := (Void).
+Definition from_void {A} (v : ∅) : A := match v with end.
 
 Class Functor (F : Type → Type) :=
   { fmap : ∀ {A B}, (A → B) → F A → F B
